describe and test semantics for state

test/MLList.lean
@@ -1,5 +1,7 @@
 import Std.Data.MLList.IO
+import Std.Data.MLList.Meta
 import Std.Tactic.GuardMsgs
+import Std.Tactic.RunCmd
 
 set_option linter.missingDocs false
 
@@ -35,3 +37,43 @@ def sleeps : MLList BaseIO UInt32 := .squash fun _ => do
 /-- info: [1, 10, 100] -/
 #guard_msgs in
 #eval sleeps.force
+
+/-!
+### Test `runGreedily`
+
+We verify that the monadic state at the completion of each job is available.
+
+We run in parallel 5 jobs which create different numbers of subgoals.
+We then sequentially count in each resulting state how many subgoals there are.
+-/
+open Lean Lean.Elab.Tactic Lean.Elab.Term
+
+def job (n : Nat) : TacticM Unit := do
+  evalTactic (← `(tactic| sleep $(quote (100*n)); iterate $(quote n) have : Nat := ?_))
+
+def runGreedily : MLList TacticM Unit :=
+  .squash fun _ => return (← TacticM.runGreedily ((List.range 5).map job)).2
+
+def runGreedilyGoals := (runGreedily.mapM fun _ => return (← getGoals).length).force
+
+/-- info: [1, 2, 3, 4, 5] -/
+#guard_msgs in
+example : True := by
+  run_tac do logInfo s!"{← runGreedilyGoals}"
+  -- It's nondeterministic which result we "end up in",
+  -- although there should be at least one `Nat` subgoal.
+  trivial
+  exact 0
+  all_goals exact 0
+
+-- We check the examples from the doc-strings extracting the state after running greedily.
+open Core Meta
+
+example (jobs : List (CoreM α)) : MLList CoreM (α × Core.State) :=
+  .squash fun _ => return (← CoreM.runGreedily jobs).2.mapM fun a => return (a, ← get)
+example (jobs : List (MetaM α)) : MLList MetaM (α × Meta.State) :=
+  .squash fun _ => return (← MetaM.runGreedily jobs).2.mapM fun a => return (a, ← get)
+example (jobs : List (TermElabM α)) : MLList TermElabM (α × Elab.Term.State) :=
+  .squash fun _ => return (← TermElabM.runGreedily jobs).2.mapM fun a => return (a, ← get)
+example (jobs : List (TacticM α)) : MLList TacticM (α × Elab.Tactic.State) :=
+  .squash fun _ => return (← TacticM.runGreedily jobs).2.mapM fun a => return (a, ← get)
